Make an area script, which does not yet work
It produces

  render% .lake/build/bin/area
  INTERNAL PANIC: unreachable code has been reached

Hopefully it's the same as https://github.com/leanprover-community/mathlib4/pull/32225.
I'm going to update Mathlib to see.

Render/Area.lean
@@ -15,6 +15,25 @@ import Render.Potential
   | .large => max 0 (p.p.scaleB (-2) * (1 - p.p.sqr) / p.dp).lo  -- Rule out a disk using Koebe
   | _ => 0  -- With .nan or .small, we give up and return the empty disk
 
+def Dyadic.toFloat : Dyadic → Float
+  | .zero => 0
+  | .ofOdd n k _ => (Float.ofInt n).scaleB (-k)
+
+instance : Lean.ToJson Dyadic where
+  toJson x := x.toFloat.toJson
+
+/-- The trace of an area computation -/
+inductive Trace where
+  | leaf : Trace
+  | free : (x y s r : Dyadic) → Trace
+  | split : (x y s r : Dyadic) → Trace → Trace → Trace → Trace → Trace
+  | leafs : (x y s r : Dyadic) → Trace  -- Same as `split` with four implicit leaves
+deriving Lean.ToJson
+
+def Trace.split' (x y s r : Dyadic) (t0 t1 t2 t3 : Trace) : Trace := match t0, t1, t2, t3 with
+  | .leaf, .leaf, .leaf, .leaf => .leafs x y s r
+  | _, _, _, _ => .split x y s r t0 t1 t2 t3
+
 /-- Upper bound the area of the Mandelbrot set contained within the square `(x,y) + [-s, s]²` -/
 def upper_area_square (x y s : Dyadic) (d n : ℕ) : Dyadic := match d with
   | 0 => 4 * s * s
@@ -27,6 +46,43 @@ def upper_area_square (x y s : Dyadic) (d n : ℕ) : Dyadic := match d with
     let u := fun dx dy ↦ upper_area_square (x + dx) (y + dy) h d n
     u h h + u (-h) h + u h (-h) + u (-h) (-h)
 
+/-- Same as `upper_area_square`, but record the samples used -/
+def upper_area_square_sample (x y s : Dyadic) (d n : ℕ) : Dyadic × Trace := match d with
+  | 0 => (4 * s * s, .leaf)
+  | d + 1 =>
+    -- Try to rule out the entire square, in which case our area bound is 0
+    let r := (free_radius ⟨.ofDyadic x, .ofDyadic y⟩ n).vald
+    if 2 * s * s ≤ r * r then (0, .free x y s r) else
+    -- Otherwise, sum across the four child squares
+    let h := div2 s
+    let u := fun dx dy ↦ upper_area_square_sample (x + dx) (y + dy) h d n
+    let (a0, t0) := u h h
+    let (a1, t1) := u (-h) h
+    let (a2, t2) := u h (-h)
+    let (a3, t3) := u (-h) (-h)
+    (a0 + a1 + a2 + a3, .split' x y s r t0 t1 t2 t3)
+
 /-- Upper bound the area of the Mandelbrot set -/
 @[irreducible] def upper_area (d n : ℕ) : Dyadic :=
   upper_area_square 0 0 2 d n
+
+/-- Same as `upper_area`, but record the samples used -/
+@[irreducible] def upper_area_sample (d n : ℕ) : Dyadic × Trace :=
+  upper_area_square_sample 0 0 2 d n
+
+/-!
+### The trace versions are the same as the non-trace versions
+-/
+
+variable {x y s : Dyadic} {d n : ℕ}
+
+@[simp] lemma fst_upper_area_square_sample :
+    (upper_area_square_sample x y s d n).1 = upper_area_square x y s d n := by
+  induction' d with d h generalizing x y s
+  · rfl
+  · simp only [upper_area_square_sample, upper_area_square, h, apply_ite]
+    grind
+
+@[simp] lemma fst_upper_area_sample :
+    (upper_area_sample d n).1 = upper_area d n := by
+  simp only [upper_area_sample, fst_upper_area_square_sample, upper_area]
